TM/Compound/Peek.v
@@ -50,7 +50,7 @@ Section Peek.
     unfold Peek_Steps. eapply RealiseIn_monotone.
     - unfold Peek. repeat TM_Correct.
     - Unshelve. 6,9: constructor 1. all: cbn. all: try omega. 4-7: constructor. cbn. constructor.
-    - TMCrush; TMSolve 1.
+    - intros tin (yout,tout). TMCrush; TMSolve 1.
   Qed.
 
 End Peek.
