TM/LiftSigmaTau.v
@@ -263,6 +263,9 @@ End LiftSigmaTau.
 Arguments Lift : simpl never.
 
 
+(** * Tactical support *)
+
+
 Ltac smpl_TM_LiftSigma :=
   match goal with
   | [ |- Lift _ _ _ _ ⊫ _] => eapply Lift_WRealise; swap 1 2
@@ -270,3 +273,12 @@ Ltac smpl_TM_LiftSigma :=
   | [ |- projT1 (Lift _ _ _ _) ↓ _] => eapply Lift_TerminatesIn; swap 1 2
   end.
 Smpl Add smpl_TM_LiftSigma : TM_Correct.
+
+
+Ltac smpl_Rel_LiftSigma :=
+  match goal with
+  | [ H : lift_sigma_tau_p _ _ _ |- _] => hnf in H
+  | [ H : lift_sigma_tau_T _ _ _ |- _] => hnf in H
+  end.
+
+Smpl Add smpl_Rel_LiftSigma : smpl_Rel.
